TM/Basic/WriteString.v
@@ -4,11 +4,11 @@ Section Write_String.
 
   Variable sig : finType.
   Variable D : move.
-  
+
   Fixpoint Write_String (l : list sig) : {M : mTM sig 1 & states M -> unit} :=
     match l with
     | [] => mono_Nop sig tt
-    | e :: l0 => Write e ;; Move _ D ;; Write_String l0
+    | e :: l0 => Write e tt ;; Move _ D tt ;; Write_String l0
     end.
 
   Fixpoint Tape_Write_String (t : tape sig) (str : list sig) :=
@@ -24,7 +24,7 @@ Section Write_String.
   Fixpoint Write_string_sem_fix (str : list sig) : Rel (tapes sig 1) (unit * tapes sig 1) :=
     match str with
     | nil => mono_Nop_R tt
-    | s :: str' => Write_R s ∘ hideParam (Move_R D ∘ hideParam (Write_string_sem_fix str'))
+    | s :: str' => Write_R s tt ∘ hideParam (Move_R D tt ∘ hideParam (Write_string_sem_fix str'))
     end.
     
   Lemma Write_string_fix_Sem (str : list sig) :
@@ -52,12 +52,8 @@ Section Write_String.
     eapply RealiseIn_monotone with (k1 := 4 * (|str|)); [now apply Write_string_fix_Sem | omega | ]. 
     induction str.
     - hnf. intros x ([], y) (H1 & H2). hnf in *. subst. now rewrite Tape_Write_String_nil.
-    - intros t1 ([], t2) (([]&t3)&H1&((b&t4)&H2&H3)). hnf in H1, H2, H3. destruct_tapes. cbn in H1, H2, H3. cbn. subst.
-      specialize (IHstr _ _ H3). clear H3. cbn in IHstr. hnf in IHstr. hnf. subst.
-      destruct b.
-      + destruct H2 as (H2&(c&H2')). cbn in H2, H2'. injection H2'. intros ->. clear H2'. subst.
-        destruct h eqn:E1, str eqn:E2; cbn; auto.
-      + destruct H2 as (H2&_). cbn in H2. congruence.
+    - intros t1 ([], t2) (([]&t3)&H1&((b&t4)&H2&H3)). hnf in *. destruct H1 as [_ H1]. destruct H2 as [_ H2]. hnf in *.
+      destruct_tapes. cbn in *. cbn. subst. specialize (IHstr _ _ H3). clear H3. cbn in IHstr. hnf in IHstr. auto.
   Qed.
 
 End Write_String.
