TM/Compound/FindSymbol.v
@@ -1,0 +1,42 @@
+Require Import Prelim.
+Require Import TM.Combinators.If TM.Combinators.SequentialComposition.
+Require Import TM.TM TM.Basic.Mono.
+Require Import TM.Compound.MoveToSymbol.
+
+
+Section FindSymbol.
+  
+  Variable sig : finType.
+  Variable f : sig -> bool.
+
+  Definition FindSymbol : { M : mTM sig 1 & states M -> FinType (EqType bool)} :=
+    If (move_to_symbol f L)
+       (mono_Nop _ true)
+       (Move _ R tt ;; move_to_symbol f R).
+
+  Definition to_symbol t :=
+    match to_symbol_l f t with
+    | (true,  t') => (true, t')
+    | (false, t') => to_symbol_r f (tape_move_mono t' (None, R))
+    end.
+
+  Definition R_FindSymbol := Mk_R_p (fun t t' => t' = to_symbol t).
+
+  Lemma FindSymbol_Realise :
+    FindSymbol ⊨ R_FindSymbol.
+  Proof.
+    eapply Realise_monotone.
+    - unfold FindSymbol. eapply If_Realise.
+      + eapply move_to_symbol_l_Realise.
+      + eapply RealiseIn_Realise. eapply mono_Nop_Sem.
+      + eapply Seq_Realise.
+        * eapply RealiseIn_Realise. eapply Move_Sem.
+        * eapply move_to_symbol_r_Realise.
+    - hnf. intros tin (yout, tout). intros H. hnf in H.
+      destruct H as [H | H]; hnf in *.
+      + destruct H as (t1&H1&->&->). unfold to_symbol. now rewrite <- H1.
+      + destruct H as(t1&H1&((b&t2)&H2&H3)); hnf in *. destruct b. destruct H2 as (_&H2).
+        unfold to_symbol. rewrite <- H1. cbn. rewrite H2 in *; clear H2. destruct_tapes. now cbn in *.
+  Qed.
+
+End FindSymbol.
